minuska/theories/builtins.v
@@ -1,0 +1,201 @@
+From Minuska Require Import
+    prelude
+    spec_syntax
+.
+
+Module empty_builtin.
+
+    Inductive Emptyset : Set := .
+
+    #[export]
+    Instance emptyset_eqdec : EqDecision Emptyset.
+    Proof.
+        intros x y.
+        destruct x, y.
+    Defined.
+
+    Section sec.
+
+        Context
+            {symbol : Set}
+            {symbols : Symbols symbol}
+        .
+
+        #[export]
+        Instance β
+            : Builtin := {|
+            builtin_value
+                := Emptyset ;
+            builtin_unary_predicate
+                := Emptyset ;
+            builtin_binary_predicate
+                := Emptyset ;
+            builtin_unary_function
+                := Emptyset ;
+            builtin_binary_function
+                := Emptyset ;
+            builtin_unary_predicate_interp
+                := fun p v => match p with end ;
+            builtin_binary_predicate_interp
+                := fun p v1 v2 => match p with end ;
+            builtin_unary_function_interp
+                := fun p v => match p with end ;
+            builtin_binary_function_interp
+                := fun p v1 v2 => match p with end ;
+        |}.
+
+        #[export]
+        Program Instance Cβ
+            :
+            @ComputableBuiltins _ _ β
+        := {|
+            builtin_unary_predicate_interp_bool := fun _ _ => false ;
+            builtin_binary_predicate_interp_bool := fun _ _ _ => false ;
+        |}.
+        Next Obligation.
+            destruct p.
+        Qed.
+        Next Obligation.
+            destruct p.
+        Qed.
+        Fail Next Obligation.
+
+    End sec.
+
+End empty_builtin.
+
+Module nat_builtin.
+
+    Inductive NatUnaryP : Set := 
+    | Nat_isZero
+    | Nat_isSuccc
+    .
+
+    #[export]
+    Instance NatUnaryP_eqdec : EqDecision NatUnaryP.
+    Proof.
+        ltac1:(solve_decision).
+    Defined.
+
+    Inductive NatBinaryP : Set :=
+    | Nat_isLe
+    | Nat_isLt
+    .
+
+    #[export]
+    Instance NatBinaryP_eqdec : EqDecision NatBinaryP.
+    Proof.
+        ltac1:(solve_decision).
+    Defined.
+
+    Inductive NatUnaryF : Set :=
+    | Nat_succOf
+    | Nat_predOf
+    .
+
+    #[export]
+    Instance NatUnaryF_eqdec : EqDecision NatUnaryF.
+    Proof.
+        ltac1:(solve_decision).
+    Defined.
+
+    Inductive NatBinaryF : Set :=
+    | Nat_plus
+    | Nat_minus
+    .
+
+    #[export]
+    Instance NatBinaryF_eqdec : EqDecision NatBinaryF.
+    Proof.
+        ltac1:(solve_decision).
+    Defined.
+
+    Section sec.
+
+        Context
+            {symbol : Set}
+            {symbols : Symbols symbol}
+        .
+
+
+        Definition err
+            {T : Type}
+        := @aoo_operand symbol (option T) None
+        .
+
+        Definition b1fmap
+            {B : Type}
+            (f : B -> B)
+            (t : GroundTerm' symbol (option B))
+            : GroundTerm' symbol (option B)
+        :=
+            match t with
+            | aoo_operand x => aoo_operand (f <$> x)
+            | _ => aoo_operand None
+            end
+        .
+
+        Notation "f '<b1$>' t" := (b1fmap f t) (at level 90).
+
+        Definition b2fmap
+            {B : Type}
+            (f : B -> B -> B)
+            (t1 t2 : GroundTerm' symbol (option B))
+            : GroundTerm' symbol (option B)
+        :=
+            match t1,t2 with
+            | aoo_operand (Some z1), aoo_operand (Some z2) =>
+                aoo_operand (Some (f z1 z2))
+            | _,_ => aoo_operand None
+            end
+        .
+
+
+        #[export]
+        Instance β
+            : Builtin
+        := {|
+            builtin_value
+                := option nat ;
+            builtin_unary_predicate
+                := NatUnaryP ;
+            builtin_binary_predicate
+                := NatBinaryP ;
+            builtin_unary_function
+                := NatUnaryF ;
+            builtin_binary_function
+                := NatBinaryF ;
+            builtin_unary_predicate_interp
+                := fun p v =>
+                match p, v with
+                | Nat_isZero, aoo_operand (Some 0) => True
+                | _, _ => False
+                end ;
+
+            builtin_binary_predicate_interp
+                := fun p v1 v2 =>
+                match p, v1, v2 with
+                | Nat_isLe, (aoo_operand (Some x)), (aoo_operand (Some y))
+                => x < y
+                | _,_,_ => False
+                end ;
+
+            builtin_unary_function_interp
+                := fun p v =>
+                match p with
+                | Nat_succOf => S <b1$> v
+                | _ => err
+                end ;
+
+            builtin_binary_function_interp
+                := fun p v1 v2 =>
+                match p, v1, v2 with
+                | Nat_plus, (aoo_operand (Some x)), (aoo_operand (Some y))
+                => aoo_operand (Some (x + y))
+                | _, _, _ => err
+                end ;
+    
+        |}.
+
+    End sec.
+End nat_builtin.
