minuska/theories/default_static_model.v
@@ -3,35 +3,25 @@ From Minuska Require Import
     spec_syntax
     spec_semantics
     string_variables
-    empty_builtin
     flattened
 .
-
 
 #[export]
 Instance MySymbols : Symbols string := Build_Symbols _ _ _.
 
-#[export]
-Program Instance Σ : StaticModel := {|
-    symbol := string ;
-    variable := string ;
-    symbols :=  MySymbols;
-    variables := StringVariables ;
-|}.
-Next Obligation.
-    apply EmptyBuiltin.
-Defined.
+Section default_model.
+    Context
+        (β : Builtin)
+    .
+
+    #[export]
+    Instance default_model : StaticModel := {|
+        symbol := string ;
+        variable := string ;
+        symbols :=  MySymbols;
+        variables := StringVariables ;
+        builtin := β ;
+    |}.
 
 
-#[export]
-Program Instance CΣ : @ComputableStaticModel Σ := {|
-    builtin_unary_predicate_interp_bool := fun _ _ => false ;
-    builtin_binary_predicate_interp_bool := fun _ _ _ => false ;
-|}.
-Next Obligation.
-    destruct p.
-Qed.
-Next Obligation.
-    destruct p.
-Qed.
-Fail Next Obligation.
+End default_model.
