minuska/theories/nat_builtin.v
@@ -1,0 +1,5 @@
+From Minuska Require Import
+    prelude
+    spec_syntax
+.
+
